src/Common/Facts.v
@@ -1,0 +1,29 @@
+Require Import List Omega.
+Require Import Common.BaseTypes Common.Mem.
+
+Lemma get_all_existing_length_le:
+  forall A AEQ V (m: @mem A AEQ V) al,
+    length (get_all_existing m al) <= length al.
+Proof.
+  induction al; intros; simpl in *; eauto.
+  destruct (m a); simpl in *; eauto.
+  omega.
+Qed.
+
+Lemma firstn_rolling_hash_list_comm:
+  forall n h vl,
+    firstn n (rolling_hash_list h vl) = rolling_hash_list h (firstn n vl).
+Proof.
+  induction n; intros; simpl in *; eauto.
+  destruct vl; simpl; eauto.
+  rewrite IHn; eauto.
+Qed.
+
+Lemma firstn_hash_and_pair_comm:
+  forall n h vl,
+    firstn n (hash_and_pair h vl) = hash_and_pair h (firstn n vl).
+Proof.
+  induction n; intros; simpl in *; eauto.
+  destruct vl; simpl; eauto.
+  rewrite IHn; eauto.
+Qed.
