src/Common/Primitives.v
@@ -1,3 +1,4 @@
 Require Export List BaseTypes Mem Pred SepAuto.
 Require Export Disk CommonAutomation ListUtils Common.HoareLogic.
+Require Export Common.Facts.
 Export ListNotations.
