src/Log/Specs.v
@@ -1,0 +1,154 @@
+Require Import String Datatypes.
+Require Import Primitives BatchOperations Layer1.
+Require Import Log.Definitions.
+
+Set Nested Proofs Allowed.
+
+Instance value_eq_dec : EqDec value := value_dec.
+
+Definition encryptionmap_valid em :=
+  (forall ev k v, em ev = Some (k, v) -> ev = encrypt k v) /\
+  (forall k k' v v', em (encrypt k v) = Some (k', v') ->
+                k = k' /\ v = v').
+
+Lemma get_all_existing_encrypt_snd :
+  forall l k (em: encryptionmap),
+    encryptionmap_valid em ->
+    (forall ev, In ev (map (encrypt k) l) -> em ev <> None) ->
+    map snd (get_all_existing em (map (encrypt k) l)) = l.
+Proof.
+  induction l; simpl; intros; eauto.
+  destruct_fresh (em (encrypt k a)); simpl in *.
+  destruct p; simpl in *.
+  rewrite IHl; eauto.
+  unfold encryptionmap_valid in *; cleanup.
+  specialize H1 with (1:= D); cleanup; eauto.
+  exfalso; eapply H0; eauto.
+Qed.
+
+Lemma get_all_existing_encrypt_fst :
+  forall l k (em: encryptionmap),
+    encryptionmap_valid em ->
+    (forall ev, In ev (map (encrypt k) l) -> em ev <> None) ->
+    map fst (get_all_existing em (map (encrypt k) l)) = repeat k (length l).
+Proof.
+  induction l; simpl; intros; eauto.
+  destruct_fresh (em (encrypt k a)); simpl in *.
+  destruct p; simpl in *.
+  rewrite IHl; eauto.
+  unfold encryptionmap_valid in *; cleanup.
+  specialize H1 with (1:= D); cleanup; eauto.
+  exfalso; eapply H0; eauto.
+Qed.
+
+Theorem apply_txn_ok :
+  forall txn log_blocks hdr txn_plain_blocks (disk_data: list data) o d a,
+    let kl := fst (fst a) in
+    let em := snd (fst a) in
+    let hm := snd a in
+    let key := txn_key txn in
+    let start := txn_start txn in
+    let addr_count := addr_count txn in
+    let data_count := data_count txn in
+    let txn_blocks := firstn (addr_count+data_count) (skipn start log_blocks) in
+    let plain_addr_blocks := firstn addr_count txn_plain_blocks in
+    let plain_data_blocks := skipn addr_count txn_plain_blocks in
+    let addr_list := firstn data_count (blocks_to_addr_list plain_addr_blocks) in
+    << o, d, a >>
+      (log_inner_rep log_blocks hdr kl em hm *
+       addr_list |L> disk_data *
+       [[ length disk_data = data_count ]] *
+       [[ In txn (txn_records hdr) ]] *
+       [[ txn_blocks = map (encrypt key) txn_plain_blocks ]] *
+       [[ encryptionmap_valid em ]])
+      (apply_txn txn log_blocks)
+      << r, ar >>
+      (log_inner_rep log_blocks hdr kl em hm *
+       addr_list |L> (map_pointwise (map vsupd plain_data_blocks) disk_data) * 
+       [[ ar = a ]])%pred
+      (exists* vsl',
+          log_inner_rep log_blocks hdr kl em hm *
+          addr_list |L> vsl' *
+          [[ ar = a ]])%pred.
+Proof.
+  unfold apply_txn; intros.
+  destruct a, p; simpl fst; simpl snd.
+
+  eapply bind_ok.
+  {
+    intros.
+    eapply pre_impl.
+    eapply add_frame.
+    apply decrypt_all_ok.
+    simpl.
+    eassign (log_inner_rep log_blocks hdr l e h * firstn (data_count txn) (blocks_to_addr_list (firstn (addr_count txn) txn_plain_blocks)) |L> disk_data).
+    unfold log_inner_rep.
+    intros; cancel.
+    all: try eauto.
+    rewrite H4.
+
+    rewrite get_all_existing_encrypt_snd; eauto.
+    intros.
+    unfold cur_txns_valid in *.
+    specialize H9 with (1:= H5); cleanup.
+    rewrite H4 in *.
+    specialize H9 with (1:=H); cleanup; congruence.
+
+    unfold cur_txns_valid in *.
+    specialize H9 with (1:= H5); cleanup.
+    rewrite H4 in *.
+    rewrite map_length.
+    symmetry; apply get_all_existing_encrypt_fst; eauto.
+    intros.
+    unfold cur_txns_valid in *.
+    specialize H7 with (1:= H9); cleanup; congruence.
+  }
+
+  { intros; simpl; cancel.
+    instantiate (1:= fun ax => firstn (data_count txn) (blocks_to_addr_list (firstn (addr_count txn) txn_plain_blocks)) |L> disk_data * log_inner_rep log_blocks hdr (fst (fst ax)) (snd (fst ax)) (snd ax) ).
+    simpl; cancel. }
+  { intros; simpl; cancel. }
+
+  intros.
+  eapply bind_ok.
+  { intros.
+    eapply pre_impl.
+    eapply add_frame.
+    apply write_batch_ok.
+
+    {
+      simpl; intros; cancel.
+      repeat destruct_lifts; cleanup.
+      cancel.
+      destruct_lift H; cleanup.
+      rewrite get_all_existing_encrypt_snd; eauto.
+      cancel.
+      intros.
+      unfold log_inner_rep, cur_txns_valid in *.
+      destruct_lift H.
+      specialize H12 with (1:= H7); cleanup.
+      rewrite H6 in *.
+      specialize H10 with (1:=H1); cleanup; congruence.
+
+      destruct_lifts.
+      destruct_lift H; cleanup.
+      rewrite get_all_existing_encrypt_snd; eauto.
+
+      unfold log_inner_rep, cur_txns_valid in *.
+      destruct_lift H.
+      specialize H11 with (1:= H7); cleanup.
+      rewrite H6 in *.
+      simpl in *.    
+      rewrite skipn_length.
+      erewrite <- map_length, <- H6.
+      rewrite firstn_length_l.
+      rewrite Minus.minus_plus; eauto.
+      rewrite skipn_length.
+      rewrite H19.
+      unfold cur_count_accurate in *.
+      rewrite H13.
+      
+      rewrite 
+      get_all_existing_length.
+    
+    
